# Recursive functions

## Basic concepts

- In Haskell, it is also permissible to define functions in terms of themselves, in which case the functions are called recursive

```hs
fac :: Int -> Int
fac 0 = 1                   -- base case
fac n = n * fac(n - 1)      -- recursive case
```
- Many functions have a simple and natural definition using recursion.  Moreover, as we shall see in chapter 16, defining functions using recursion also allows properties of those functions to be proved using the simple but powerful technique of **induction**

## Recursion on lists

- Recursion is not restricted to functions on integers, but can also be used to define functions on lists

```hs
product [] = 1
product (n:ns) = n * product ns
```

- For the usage of `n:ns`: Recall that lists in Haskell are actually constructed one element at a time using the cons operator `:`. For example, `[2, 3, 4]` is just an abbreviation for `2:(3:(4:[]))`.

```txt
product [2,3,4]
= 2 * product [3, 4]
= 2 * (3 * product [4])
= 2 * (3 * (4 * product []))
= 2 * (3 * (4 * 1))
= 24
```
- Some other examples

```hs
length [] = 0
length (_:xs) = 1 + length xs
```

```hs
reverse [] = []
reverse (x:xs) = reverse xs ++ [x]
```

```hs
[] ++ ys = ys
(x:xs) ++ ys = x : (xs ++ ys)
```

```hs
insert x []                 = [x]
insert x (y:ys) | x <= y    = x : y : ys
                | otherwise = y : insert x ys


insertion_sort [] = []
insertion_sort (x:xs) = insert x (insertion_sort xs)
```

## Multiple arguments

- Functions with multiple arguments can also be defined using recursion on more than one argument at the same time

```hs
zip [] _ = []
zip _ [] = _
zip (x:xs) (y:ys) = (x, y) : zip xs ys
```

```hs
drop 0 xs = xs
drop _ [] = []
drop n (_:xs) = drop (n - 1) xs
```

## Multiple recursion

- Functions can also be defined using multiple recursion, in which a function is applied more than once in its own definition

```hs
fib 0 = 0
fib 1 = 1
fib n = fib (n - 2) + fib (n - 1)
```

```hs
qsort [] = []
qsort (x:xs) = qsort smaller ++ [x] ++ qsort larger
               where
                 smaller = [a | a <- xs, a <= x]
                 larger = [b | b <- xs, b > x]
```

## Mutual recursion

- mutual recursion: two or more functions are all defined recursively in terms of each other.

```hs
-- for non-negative integers
even 0 = True
even n = odd (n - 1)

odd 0 = False
odd n = even (n - 1)
```

- Similarly, functions that select the elements from a list at all even and odd positions (counting from zero) can be defined as:

```hs
evens [] = []
evens (x:xs) = x : odds xs

odds [] = []
adds (_:xs) = evens xs
```

- so it works like:

```txt
evens "abcde"
= 'a' : odds "bcde"
= 'a' : evens "cde"
= 'a' : ('c' : odds "de")
= 'a' : ('c' : evens "e")
= 'a' : ('c' : ('e' : odds []))
= "ace"
```

## Advice on recursion

Step 1: define the type

- Thinking about types is very helpful when defining functions, so it is good practice to define the type of a function prior to starting to define the function itself

```hs
product :: [Int] -> Int
```

Step 2: enumerate the cases

- For most types of argument, there are a number of standard cases to consider.
- For lists, the standard cases are the empty list and non-empty lists

```hs
product :: [Int] -> Int
product []     = ...?
product (n:ns) = ...?
```

- For non-negative integers, the standard cases are 0 and n, for logical values they
are False and True, and so on


Step 3: define the simple cases

- The simple cases often become base cases.

```hs
product :: [Int] -> Int
product []     = 1
product (n:ns) = ...?
```

Step 4: define the other cases

- First consider the ingredients that can be used, such as
  - the function itself (`product`),
  - the arguments (`n` and `ns`), and
  - library functions of relevant types (`+`, `-`, `*`, and so on.)

```hs
product :: [Int] -> Int
product []     = 1
product (n:ns) = n * product ns
```

Step 5: generalize and simplify

- Once a function has been defined using the above process, it often becomes clear that it can be generalized and simplified
- For example, the function `product` does not depend on the precise kind of numbers to which it is applied.

```hs
product :: Num a => [a] -> a
product []     = 1
product (n:ns) = n * product ns
```

- One step further, the pattern of recursion used in `product` is encapsulated by a library function called `foldr`. And can be defined as:

```hs
product :: Num a => [a] -> a
product = foldr (*) 1
```

## Example: `drop`

- Goal: an expression of the form `drop n xs`: drop `n` elements from `xs`

```hs
drop :: Integral b => b -> [a] -> [a]
drop 0 [] = []
drop 0 (x:xs) = (x:xs)
drop n [] = []
drop n (x:xs) = drop (n-1) xs
```

- and simplify more

```hs
drop :: Integral b => b -> [a] -> [a]
drop 0 xs = xs
drop _ [] = []
drop n (x:xs) = drop (n-1) xs
```

## Example: `init`

- Goal: removes the last element from a non-empty list

```hs
init :: [a] -> [a]
init [_] = []
init (x:xs) = x : init xs
```